ocaml2zoo/lib/zoo/syntax.mli
@@ -13,10 +13,8 @@ type tag =
 type rec_flag =
   Asttypes.rec_flag
 
-type concreteness =
-  | Concrete
-  | Abstract
-  | Revealed
+type mutable_flag =
+  Asttypes.mutable_flag
 
 type typ =
   | Type_product of field list
@@ -56,7 +54,8 @@ type expression =
   | Tuple of expression list
   | Ref of expression
   | Record of expression list
-  | Constr of concreteness * tag * expression list
+  | Constr of mutable_flag * tag * expression list
+  | Reveal of expression
   | Proj of expression * field
   | Match of expression * branch list * fallback option
   | Ref_get of expression
